TCSlib.lean
@@ -22,6 +22,7 @@ import TCSlib.CommunicationComplexity.NewmanTheorem
 
 import TCSlib.Complexity.NPReductions
 import TCSlib.Complexity.TuringMachine
+import TCSlib.Complexity.Uncomputability
 import TCSlib.Complexity.ClassP
 
 import TCSlib.Cryptography.SchnorrProtocol
